veric/extend_tc.v
@@ -393,10 +393,17 @@ Proof. solve_proper. Qed.
    small-footprint approach to the environment, while tc_expr and eval_expr freely
    call on the full environment rho. So to do this, we need to first fix the entire
    environment. *)
+
 Definition curr_env (ge : genv) f (rho : environ) : mpred.assert :=
   <affine> ⌜(stack_size f = O -> te_of rho = ∅) ∧ ∀ i, Map.get (ge_of rho) i = Genv.find_symbol ge i⌝ ∗
-  ⎡own(inG0 := envGS_inG) env_name (lib.gmap_view.gmap_view_auth dfrac.DfracDiscarded (to_agree <$> make_env (Genv.genv_symb ge)), ε)⎤ ∗
+  ⎡globals_auth (make_env (Genv.genv_symb ge))⎤ ∗
   assert_of' (λ n, stack_frag n (stack_frac f) 1%Qp (ve_of rho) (te_of rho)).
+
+Lemma curr_env_ge : forall ge f rho, curr_env ge f rho ⊢ curr_env ge f rho ∗
+   <affine> ⌜∀ i : ident, Map.get (ge_of rho) i = Genv.find_symbol ge i⌝ ∗ ⎡globals_auth (make_env (Genv.genv_symb ge))⎤.
+Proof.
+  intros; iIntros "((% & %) & #$ & $)"; auto.
+Qed.
 
 Lemma curr_env_e : forall ρ ge0 f rho, ⊢ ⎡env_auth ρ⎤ -∗ curr_env ge0 f rho -∗
   □ ∀ ge ve te, env_match ρ ge ve te -∗ ⌜Genv.find_symbol ge0 = Genv.find_symbol ge /\ env_matches rho ge0 ve te⌝.
@@ -423,11 +430,10 @@ Qed.
 
 Lemma curr_env_gvar_e : forall ge f rho i b, curr_env ge f rho ∗ ⎡gvar i b⎤ ⊢ ⌜Genv.find_symbol ge i = Some b⌝.
 Proof.
-  intros; rewrite /gvar /curr_env.
-  iIntros "(((_ & %H) & H1 & _) & H2)"; iDestruct (own_valid_2 with "H1 H2") as %((? & _ & _ & Hid & _ & Hincl)%gmap_view.gmap_view_both_dfrac_valid_discrete_total & _).
-  rewrite lookup_fmap in Hid; specialize (H i); destruct (lookup _ _) eqn: Hi; inv Hid.
-  rewrite make_env_spec in Hi.
-  by apply to_agree_included_L in Hincl as ->.
+  intros; rewrite /curr_env.
+  iIntros "((% & ? & _) & ?)".
+  iDestruct (globals_gvar_e with "[$]") as %Hi.
+  rewrite make_env_spec in Hi; auto.
 Qed.
 
 Lemma curr_env_set_temp : forall Delta ge f rho i t
